src/StVM.v
@@ -5,20 +5,16 @@ Author:  Adam Petz, ampetz@ku.edu
 *)
 
 Require Import ConcreteEvidence.
-Require Import Maps.
 Require Import List.
 Import ListNotations.
 
-Definition Event_ID := nat.
+Definition Event_ID: Set := nat.
 
 (* Specific VM monad state *)
-(*Definition ev_store := MapC nat EvidenceC. *)
 Record cvm_st : Type := mk_st
                           {st_ev:EvC ;
                            st_trace:list Ev ;
                            st_pl:Plc;
-                           st_evid:Event_ID
-                           (*;
-                           st_store:ev_store*)}.
+                           st_evid:Event_ID}.
 
-Definition empty_vmst := mk_st (evc [] mt) [] 0 0 (* [] *) .
+Definition empty_vmst := mk_st (evc [] mt) [] 0 0.
